\begin{tiny}(Ccp33)\end{tiny} Avec les notations de l'énoncé,
\[
 ax + by = a\Re z + b \Im z.
\]
Cela fait penser à
\[
 \Re(zz') = \Re z \Re z' - \Im z \Im z'
\]
ou plutôt à
\[
 \Re(z\overline{z'}) = \Re z \Re z' + \Im z \Im z'.
\]
Considérons $a + i b$ et nommons le $w$. Alors
\[
 ax + by + c = \Re(z\overline{w} + c).
\]
Considérons $-\frac{c}{\overline{w}}$ et nommons le $u$: alors $c = -\overline{w} u$ et
\[
 ax + by +c = \Re\left( z\overline{w} - u \overline{w}\right) = \Re\left( (z-u)\overline{w}\right).  
\]
