\begin{tiny}(Cde11)\end{tiny} Notons 
\begin{displaymath}
 f(x)= \ln\left( \sum_{k=0}^{99}\frac{x^k}{k!}\right)
\end{displaymath}
D'après le développement en $0$ de l'exponentielle à l'ordre $101$:
\begin{multline*}
 f(x)=\ln\left(e^x -\frac{x^{100}}{100!}-\frac{x^{101}}{101!} +o(x^{101})\right) \\
= x+\ln\left(1 -e^{-x}\frac{x^{100}}{100!}-e^{-x}\frac{x^{101}}{101!} +o(x^{101})\right)
\end{multline*}

car $e^{-x}\rightarrow 1$ entraîne $o(e^{-x}x^{101})=o(x^{101})$. De plus,
\begin{align*}
 e^{-x}\frac{x^{101}}{101!}&= \frac{x^{101}}{101!} +o(x^{101})\\
 e^{-x}\frac{x^{100}}{100!}&= \frac{x^{100}}{100!}-\frac{x^{101}}{100!} +o(x^{101})
\end{align*}
On en déduit
\begin{multline*}
 f(x)=x+\ln\left(1- \frac{x^{100}}{100!}+\frac{100\,x^{101}}{101!}+o(x^{101})\right)\\
 = x - \frac{x^{100}}{100!}+\frac{100\,x^{101}}{101!}+o(x^{101})
\end{multline*}

