\begin{tiny}(di35)\end{tiny} Formons des théorèmes du rang: 
\begin{align*}
\dim E_0 &= \dim (\Im f_0) + \dim (\ker f_0) &\times (-1)^0 \\  
\dim E_1 &= \dim (\Im f_1) + \dim (\ker f_1) &\times (-1)^1 \\
\dim E_2 &= \dim (\Im f_2) + \dim (\ker f_2) &\times (-1)^2  \\
 & \vdots \\
 \dim E_n &= \dim (\Im f_n) + \dim (\ker f_n) &\times (-1)^n
\end{align*}
On somme en tenant compte de $\Im f_i = \ker f_{i+1}$:
\begin{multline*}
  \sum_{i=0}^n (-1)^{i}\dim E_i = \dim (\ker f_0) + (-1)^n\Im f_{n}\\
  = (-1)^n \dim E_{n+1}
\end{multline*}

car $f_0$ est injective et $f_n$ est surjective. On en déduit
\[
  \sum_{i=0}^{n+1} (-1)^{i}\dim E_i = 0.
\]
