\begin{tiny}(Cee26)\end{tiny} Pour tout $x\in G^\bot$, il existe $(f,g)\in F \times G$ tels que $x=f+g$. Alors:
\[
 (g/g) = (g/ x - f) = (\underset{\in G}{g}/ \underset{\in G^\bot}{x}) - (\underset{\in G}{g}/ \underset{\in F \subset G^\bot}{f})
 = 0 
\]
donc $G^\bot \subset F$. On sait que $G \subset G^{\bot \bot}$. D'autre part,
\[
 F \subset G^\bot \Rightarrow G^{\bot \bot} \subset F^\bot \Rightarrow G \subset F^\bot.
\]
On termine comme plus haut. Pour tout $x\in F^\bot$, il existe $(f,g)\in F\times G$ tels que $x=f=g$. Alors
\[
 (f/f) = (f/ x - g) = (\underset{\in F}{f}/ \underset{\in F^\bot}{x}) - (\underset{\in F}{f}/ \underset{\in G \subset F^\bot}{g})
 = 0 .
\]
Donc $F^\bot \subset G$.