\begin{tiny}(Cmf17)\end{tiny} L'énoncé se traduit par
\begin{displaymath}
 a = e_1 + e_2 + e_3,\; b = e_1 + e_3,\; c = e_1+2e_2+3e_3
\end{displaymath}
 Comme $p$ est la projection sur $\Vect(a)$ parallèlement à $\Vect(b,c)$, on en tire
\begin{displaymath}
 e_2 = a-b \Rightarrow p(e_2)= a
\end{displaymath}
\begin{displaymath}
 c-a = e_2 +2e_3 \Rightarrow -a= a + 2p(e_3)\Rightarrow p(e_3)=-a
\end{displaymath}
\begin{displaymath}
 p(b)=0 \Rightarrow p(e_1)=-p(e_3)=a 
\end{displaymath}
Comme $a=e_1+e_2+e_3$, la matrice demandée est
\begin{displaymath}
 \begin{pmatrix}
  1 & 1 & -1 \\1 & 1 & -1 \\ 1 & 1 & -1
 \end{pmatrix}
\end{displaymath}
 