\begin{tiny}(Csc28)\end{tiny}
On remarque d'abord que 
\[
 \sqrt{n} \leq \sqrt{n+1} \Rightarrow u_n \leq v_n.
\]
Ensuite:
\begin{multline*}
 u_{n+1} - u_n
 = \frac{1}{\sqrt{n+1}} -2\sqrt{n+2} + 2\sqrt{n+1}\\
 = \frac{1}{\sqrt{n+1}} - \frac{2}{\underset{> 2\, \sqrt{n+1}}{\underbrace{\sqrt{n+2} + \sqrt{n+1}}}}
 > 0 .
\end{multline*}
De mÃªme,
\begin{multline*}
 v_{n+1} - v_n
 = \frac{1}{\sqrt{n+1}} -2\sqrt{n+1} + 2\sqrt{n}\\
 = \frac{1}{\sqrt{n+1}} - \frac{2}{\underset{< 2\, \sqrt{n+1}}{\underbrace{\sqrt{n+1} + \sqrt{n}}}}
 < 0 .
\end{multline*}
Enfin,
\begin{multline*}
 v_n - u_n = 2\left( \sqrt{n+1} - \sqrt{n}\right)
 = \frac{2}{\sqrt{n+1} + \sqrt{n}} \rightarrow 0.
\end{multline*}
Les deux suites sont donc adjacentes.