\begin{tiny}(Csc32)\end{tiny}
\[
  \forall n \geq 2, 
  u_{n+1} - u_n = \frac{1}{n^2(n+1)^2} > 0.
\]
Donc $(u_n)_{n\in \N^*}$ croissante.
\begin{multline*}
  \forall n \geq 2, 
  v_{n+1} - v_n = \frac{1}{n^2(n+1)^2} + \frac{1}{3(n+1)^2} - \frac{1}{3n^2}\\
  = \frac{3 + n^2 - (n+1)^2}{3 n^2(n+1)^2}
  = \frac{2 - 2n}{3 n^2(n+1)^2} < 0.
\end{multline*}

Donc $(v_n)_{n\in \N^*}$ décroissante.
\[
  \forall n \geq 2, v_n - u_n = \frac{1}{3n^2}.
\]
Donc $(v_n - u_n)_{n\in \N^*}$ décroit et converge vers $0$. Les suites sont adjacentes.
